cbor_raw_slice_iterator_init

src/cbor/raw/pulse/CBOR.Pulse.Raw.Util.fst
@@ -1,6 +1,10 @@
 module CBOR.Pulse.Raw.Util
 open Pulse.Lib.Pervasives
 
+// FIXME: this file is VERY brittle
+
+let perm_div (p1 p2: perm) : Tot perm = p1 /. p2
+
 let perm_mul (p1 p2: perm) : Tot perm = p1 *. p2
 
 #reset-options "--smtencoding.elim_box true --smtencoding.l_arith_repr native --smtencoding.nl_arith_repr native"
@@ -23,4 +27,8 @@ let perm_1_l
 
 let half_mul (a b: real) : Lemma
   ((a *. b) /. 2.0R == a *. (b /. 2.0R))
+= ()
+
+let perm_mul_div (a b: perm) : Lemma
+  (a `perm_mul` (b `perm_div` a) == b)
 = ()
